fix issues related to name mangling of rules inside private rule instances

Heron/Refactor/Inline/Detects.lean
@@ -16,3 +16,17 @@ def myConst :=
 #assertRefactor inline in
 example : Nat := myConst
 becomes `(example : Nat := (42))
+
+meta def metaDouble (n : Nat) :=
+  n + n
+
+#assertRefactor inline in
+example : Nat := metaDouble 3
+becomes `(example : Nat := (3 + 3))
+
+private def privateConst :=
+  7
+
+#assertRefactor inline in
+example : Nat := privateConst
+becomes `(example : Nat := (7))
