Heron/Refactor/InlineAll/Detects.lean
@@ -11,3 +11,21 @@ def triple (n : Nat) :=
     triple 2 + triple 3 becomes
   `(example : Nat :=
       (2 + 2 + 2) + (3 + 3 + 3))
+
+meta def metaAdd (a b : Nat) :=
+  a + b
+
+#assertRefactor inlineAllConst in
+  example : Nat :=
+    metaAdd 1 2 + metaAdd 3 4 becomes
+  `(example : Nat :=
+      (1 + 2) + (3 + 4))
+
+private def privateAdd (a b : Nat) :=
+  a + b
+
+#assertRefactor inlineAllConst in
+  example : Nat :=
+    privateAdd 1 2 + privateAdd 3 4 becomes
+  `(example : Nat :=
+      (1 + 2) + (3 + 4))
